scripts/asm-fixtures/witnessCodesIndexBuildFunction.s
@@ -1,0 +1,139 @@
+witness_codes_index_build:
+  addi x2, x2, -96
+  sd x1, 0(x2)
+  sd x8, 8(x2)
+  sd x9, 16(x2)
+  sd x18, 24(x2)
+  sd x19, 32(x2)
+  sd x20, 40(x2)
+  sd x21, 48(x2)
+  sd x22, 56(x2)
+  sd x23, 64(x2)
+  sd x24, 72(x2)
+  sd x25, 80(x2)
+  la x5, wcidx_enabled
+  sd x0, 0(x5)
+  mv x8, x10
+  mv x9, x11
+  la x5, wcidx_build_status
+  sd x0, 0(x5)
+  la x5, wcidx_build_section_len
+  sd x9, 0(x5)
+  la x5, wcidx_build_count
+  sd x0, 0(x5)
+  la x5, wclh_lookup_calls
+  sd x0, 0(x5)
+  la x5, wclh_indexed_calls
+  sd x0, 0(x5)
+  la x5, wclh_indexed_hits
+  sd x0, 0(x5)
+  la x5, wclh_indexed_misses
+  sd x0, 0(x5)
+  la x5, wclh_linear_calls
+  sd x0, 0(x5)
+  la x5, wclh_linear_hits
+  sd x0, 0(x5)
+  la x5, wclh_linear_misses
+  sd x0, 0(x5)
+  la x5, wclh_linear_iterations
+  sd x0, 0(x5)
+  la x5, wclh_linear_last_section_len
+  sd x0, 0(x5)
+  la x5, wclh_linear_max_section_len
+  sd x0, 0(x5)
+  beq x9, x0, .+168
+  li x5, 4
+  bltu x9, x5, .+328
+  lwu x5, 0(x8)
+  andi x6, x5, 3
+  bne x6, x0, .+316
+  bltu x9, x5, .+312
+  srli x18, x5, 2
+  la x6, wcidx_build_count
+  sd x18, 0(x6)
+  lui x6, 0x20
+  bltu x6, x18, .+288
+  mv x19, x5
+  li x20, 0
+  beq x20, x18, .+112
+  slli x5, x20, 2
+  add x6, x8, x5
+  lwu x21, 0(x6)
+  bltu x21, x19, .+260
+  bltu x9, x21, .+256
+  addi x7, x20, 1
+  beq x7, x18, .+24
+  slli x28, x7, 2
+  add x28, x8, x28
+  lwu x22, 0(x28)
+  bltu x9, x22, .+232
+  jal x0, .+8
+  mv x22, x9
+  bltu x22, x21, .+220
+  sub x23, x22, x21
+  mv x10, x20
+  jal x1, wcidx_record_ptr
+  mv x24, x10
+  add x10, x8, x21
+  mv x11, x23
+  mv x12, x24
+  jal x1, zkvm_keccak256
+  sd x21, 32(x24)
+  sd x23, 40(x24)
+  addi x20, x20, 1
+  jal x0, .-104
+  li x18, 0
+  li x5, 2
+  bltu x18, x5, .+100
+  srli x20, x18, 1
+  beq x20, x0, .+24
+  addi x20, x20, -1
+  mv x10, x20
+  mv x11, x18
+  jal x1, wcidx_sift_down
+  jal x0, .-20
+  mv x20, x18
+  li x5, 1
+  bgeu x5, x20, .+60
+  addi x20, x20, -1
+  li x10, 0
+  jal x1, wcidx_record_ptr
+  mv x24, x10
+  mv x10, x20
+  jal x1, wcidx_record_ptr
+  mv x25, x10
+  mv x10, x24
+  mv x11, x25
+  jal x1, wcidx_swap_records
+  li x10, 0
+  mv x11, x20
+  jal x1, wcidx_sift_down
+  jal x0, .-60
+  la x5, wcidx_section_ptr
+  sd x8, 0(x5)
+  la x5, wcidx_section_len
+  sd x9, 0(x5)
+  la x5, wcidx_count
+  sd x18, 0(x5)
+  li x6, 1
+  la x5, wcidx_enabled
+  sd x6, 0(x5)
+  li x10, 0
+  jal x0, .+24
+  li x6, 1
+  la x5, wcidx_build_status
+  sd x6, 0(x5)
+  li x10, 1
+  ld x1, 0(x2)
+  ld x8, 8(x2)
+  ld x9, 16(x2)
+  ld x18, 24(x2)
+  ld x19, 32(x2)
+  ld x20, 40(x2)
+  ld x21, 48(x2)
+  ld x22, 56(x2)
+  ld x23, 64(x2)
+  ld x24, 72(x2)
+  ld x25, 80(x2)
+  addi x2, x2, 96
+  jalr x0, 0(x1)
